\documentclass[a4paper, 12pt, twoside]{article}
\usepackage[left = 3cm, right = 3cm]{geometry}
\usepackage[english]{babel}
\usepackage[utf8]{inputenc}
\usepackage{amssymb}
\usepackage{amsmath}
\usepackage{amsthm}
\usepackage{multicol}

\author{Joseph}

\begin{document}
Joseph Dowling.
\subsection*{Exercise 1.a)}


\subsection*{Exercise 3}
We have that $(fg)'=fg'+f'g$ so $\int_{\gamma}(fg)'=\int_{\gamma}fg'+\int_{\gamma}f'g$ and then by the fundamental theorem we have
$$\int_{\gamma}(fg)'=f(b)g(b)-f(a)g(a) $$
Combining our two equations we get
$$\int_{\gamma}fg'+\int_{\gamma}f'g=f(b)g(b)-f(a)g(a) $$
Then rearanging
$$\int_{\gamma}fg'=f(b)g(b)-f(a)g(a)-\int_{\gamma}f'g$$
\subsection*{Exercise 5}
We have $L(\gamma)=\int_{0}^{2\pi}|\gamma'(t)|dt=\int_{0}^{2\pi}|ie^{it}|dt=2\pi $. And we also have
\begin{align*}
    \sup_{t}|\frac{\sin(\gamma(t))}{\gamma(t)^{2}}| &= \sup_{t} |\frac{e^{i\gamma(t)}-e^{-i\gamma(t)}}{2i\gamma(t)^{2}}| \\
    & = \sup_{t} \frac{|e^{i\gamma(t)}-e^{-i\gamma(t)}|}{|2i\gamma(t)^{2}|}\\
    & \leq \sup_{t} \frac{|e^{i\gamma(t)}|+|e^{-i\gamma(t)}|}{|2i\gamma(t)^{2}|}\\
    &= \sup_{t} \frac{1}{|\gamma(t)|^{2}} = 1?
\end{align*}
Then by the estimation lemma we get
$$|\int_{\gamma}\frac{\sin(z)}{z^{2}}dz|\leq 2\pi e $$
\subsection*{Exercise 6)}
\begin{itemize}
    \item[b)]
    \item[c)]
\end{itemize}

\end{document}
