\documentclass[a4paper, 12pt, twoside]{article}
\usepackage[left = 3cm, right = 3cm]{geometry}
\usepackage[english]{babel}
\usepackage[utf8]{inputenc}
\usepackage{amssymb}
\usepackage{amsmath}
\usepackage{amsthm}
\usepackage{multicol}

\author{jdRanda}

\begin{document}
\subsection*{Exercise 1.b)}
\begin{align*}
    |z+w|^{2} &= |z^{2}|+2zw+|w^{2}|\\
    &\leq |z|^{2}+|w|^{2}\\
    &\leq (|z|+|w|)^{2}\\
    |z+w| &\leq|z|+|w|
\end{align*}
\subsection*{Exercise 4}
\begin{itemize}
    \item[a)]
    Suppose $z\in \mathbb{C}, z\neq0$, then $f(z)=\frac{z^{4}}{|z|^{2}}= \frac{z^{4}}{\overline{z}z}$. Hence applying lemma 2.22 we have
    $$\frac{\partial}{\partial\overline{z}}f(z)=\frac{-z^{3}}{\overline{z}^{2}}\neq 0\text{   for } z \neq 0$$
    Now suppose $z=0\in \mathbb{C}$, let $h\in \mathbb{C}$, then
    $$ \lim_{h\to0}\frac{f(0+h)-f(0)}{h}=\lim_{h\to0}\frac{\frac{h^{3}}{\overline{h}}}{h}= \lim_{h\to0}\frac{h^{2}}{\overline{h}}=0 $$
    Hence $f$ is complex differentiable at $z=0$.
    \item[b)]
    From our function $f(z)=2xy+i(x+\frac{2}{3}y^{3})$ we have $u(x,y)=2xy,v(x,y)= x+\frac{2}{3}y^{3}$ which are both trivially continious as they are polynomials. So we have
    $$u_{x}=2y,u_{y}=2x,v_{x}=1,v_y=2y^{2} $$
    Hence for
    \begin{align*}
        u_{x}=2y &= v_y=2y^{2}\\
        u_{y}=2x &= -v_{x}=-1
    \end{align*}
    The only solutions are $z=0,z=-\frac{1}{2}$.
\end{itemize}

\newpage
\subsection*{Exercise 7,a)}
We prove directly from the definition of the derivative. We already know
$$ \lim_{h\to0}\frac{f(z+h)-f(z)}{h}=f'(z)$$
and so we show
\begin{align*}
    \lim_{h\to0}\frac{g(z+h)-g(z)}{h} &=
    \lim_{h\to0}\frac{\overline{f(\overline{z+h})}-\overline{f(\overline{z})}}{h}\\
    &= \lim_{h\to0}\frac{\overline{f(\overline{z}+\overline{h})-{f(\overline{z})}}}{h}\\
    &=\overline{\lim_{h\to0}\frac{f(\overline{z}+\overline{h})-{f(\overline{z})}}{\overline{h}}}\\
    &=\overline{f'(\overline{z})}<\infty
\end{align*}
Hence g is complex differentiable at $z$.


\subsection*{Exercise 9}



\subsection*{Exercise 10}
Let $f(z)=z^{3}$, $z=x+iy, x,y\in \mathbb{R}$. Then
$$ f(z)=(x+iy)^{3}=x^{3}+3x^{2}iy-3xy^{2}-iy^{3}$$
and so we have that
$$Re(f)= x^{3}-3xy^{2}$$
\end{document}
